Test/Issues/Trust.lean
@@ -1,0 +1,4 @@
+import Smt
+
+example : True := by
+  smt +trust
